updates

Veritas.MultiSet.fst
@@ -4,7 +4,7 @@ let mset (a:eqtype):Type0 = admit()
 
 let mem (#a:eqtype) (x:a) (s:mset a): Tot nat = admit()
 
-let equal (#a:eqtype) (s1:mset a) (s2:mset a): Tot bool = admit()
+let equal (#a:eqtype) (s1:mset a) (s2:mset a): Tot prop = admit()
 
 let lemma_eq_intro (#a:eqtype) (s1 s2:mset a): 
   Lemma (requires (forall (x:a). (mem x s1 = mem x s2)))
@@ -21,14 +21,8 @@ let lemma_eq_elim (#a:eqtype) (s1 s2: mset a):
 (* empty set *)
 let empty (#a:eqtype): Tot (mset a) = admit()
 
-let lemma_empty_implies_notmem (#a: eqtype) (s: mset a) (x: a):
-  Lemma (requires (is_empty s))
-        (ensures (~ (contains s x))) = admit()
-
-let hasEq_lemma (a:Type):
-  Lemma (requires (hasEq a)) 
-        (ensures (hasEq (mset a))) 
-        [SMTPat (hasEq  (mset a))] = admit()
-
 (* construct a multiset given a sequence *)
 let seq2mset (#a:eqtype) (s: seq a): Tot (mset a) = admit()
+
+let lemma_count_mem (#a:eqtype) (s: seq a) (x: a):
+  Lemma (count x s = mem x (seq2mset s)) = admit()
