Veritas.MultiSet.fsti
@@ -8,7 +8,7 @@ val mset (a:eqtype): Type0
 val mem (#a:eqtype) (x:a) (s:mset a): Tot nat
 
 (* equality of two multisets *)
-val equal (#a:eqtype) (s1 s2:mset a): Tot bool
+val equal (#a:eqtype) (s1 s2:mset a): Tot prop
 
 val lemma_eq_intro (#a:eqtype) (s1 s2:mset a): 
   Lemma (requires (forall (x:a). (mem x s1 = mem x s2)))
@@ -25,22 +25,9 @@ val lemma_eq_elim (#a:eqtype) (s1 s2: mset a):
 (* empty set *)
 val empty (#a:eqtype): Tot (mset a)
 
-(* does a multiset contain an element x *)
-let contains (#a:eqtype) (s:mset a) (x:a) = mem x s > 0 
-
-let is_empty (#a:eqtype) (s:mset a): Tot bool = 
-  equal s empty
-
-(* the empty set does not contain anything *)
-val lemma_empty_implies_notmem (#a: eqtype) (s: mset a) (x: a):
-  Lemma (requires (is_empty s))
-        (ensures (~ (contains s x)))
-
-(* TODO: what connects boolean equality '=' and equal *)
-val hasEq_lemma (a:Type):
-  Lemma (requires (hasEq a)) 
-        (ensures (hasEq (mset a))) 
-        [SMTPat (hasEq  (mset a))]
-
 (* construct a multiset given a sequence *)
 val seq2mset (#a:eqtype) (s: seq a): Tot (mset a)
+
+(* count of an element in seq s is its membership count in its corresponding multiset *)
+val lemma_count_mem (#a:eqtype) (s: seq a) (x: a):
+  Lemma (count x s = mem x (seq2mset s))
