Veritas.Verifier.Defs.fst
@@ -7,5 +7,5 @@ let empty_hash_value = zero_vec
 let ms_hashfn_upd (e:ms_hashfn_dom) (h:ms_hash_value): ms_hash_value = admit()
 
 let lemma_mshashfn_correct (s1 s2: seq ms_hashfn_dom):
-  Lemma (requires (seq2mset s1 = seq2mset s2))
+  Lemma (requires (seq2mset s1 == seq2mset s2))
         (ensures (ms_hashfn s1 = ms_hashfn s2)) = admit()
