Veritas.Verifier.Defs.fsti
@@ -80,5 +80,6 @@ let rec ms_hashfn (s: seq ms_hashfn_dom): Tot ms_hash_value
 
 (* two sequences that encode the same multiset produce the same hash *)
 val lemma_mshashfn_correct (s1 s2: seq ms_hashfn_dom):
-  Lemma (requires (seq2mset s1 = seq2mset s2))
+  Lemma (requires (seq2mset s1 == seq2mset s2))
         (ensures (ms_hashfn s1 = ms_hashfn s2))
+
