Veritas.Verifier.fst
@@ -22,6 +22,9 @@ type vlog_entry_thread =
   | MemoryOp: o:memory_op -> vlog_entry_thread
   | AddM: a:merkle_addr -> v:merkle_payload -> a':merkle_addr -> vlog_entry_thread
   | EvictM: a:merkle_addr -> a':merkle_addr -> vlog_entry_thread
+  | AddB: a:merkle_addr -> v:merkle_payload -> t:timestamp -> vlog_entry_thread 
+  | EvictB: a:merkle_addr -> t:timestamp -> vlog_entry_thread
+  | EvictBM: a: merkle_addr -> a':merkle_addr -> t:timestamp -> vlog_entry_thread
 
 (* verifier log entry *)
 type vlog_entry = 
@@ -33,8 +36,17 @@ type vlog = seq vlog_entry
 (* index in the verifier log *)
 type vl_index (l:vlog) = seq_index l
 
+(* for records in the store, how were they added? *)
+type add_method = 
+  | Merkle: add_method       (* AddM *)
+  | Blum: add_method         (* AddB *)
+
+(* information we keep for each addr in store *)
+type vstore_payload (a:merkle_addr) = 
+  | SP: v:merkle_payload_of_addr a -> add:add_method -> vstore_payload a
+
 (* verifier store is a subset of merkle_addr, merkle_payloads *)
-type vstore = (a:merkle_addr) -> option (merkle_payload_of_addr a)
+type vstore = (a:merkle_addr) -> option (vstore_payload a)
 
 (* does the store contain address a *)
 let store_contains (store:vstore) (a:merkle_addr) = Some? (store a)
@@ -42,7 +54,10 @@ let store_contains (store:vstore) (a:merkle_addr) = Some? (store a)
 (* lookup the payload of an address in store *)
 let stored_payload (store:vstore) (a:merkle_addr{store_contains store a}):
   (merkle_payload_of_addr a) = 
-  Some?.v (store a)
+  SP?.v (Some?.v (store a))
+
+let stored_add_method (store:vstore) (a:merkle_addr{store_contains store a}): add_method = 
+    SP?.add (Some?.v (store a))
 
 (* update the store *)
 let store_update (store:vstore) 
@@ -50,24 +65,19 @@ let store_update (store:vstore)
                  (v:merkle_payload_of_addr a):
   Tot (store':vstore {store_contains store' a /\ 
                       stored_payload store' a = v}) = 
-  fun a' -> if a' = a then Some v else store a'
+  let am = stored_add_method store a in                      
+  fun a' -> if a' = a then Some (SP v am) else store a'
+
+(* add a new record to the store *)
+let store_add (s:vstore)
+              (a:merkle_addr{not(store_contains s a)})
+              (v:merkle_payload_of_addr a)
+              (am:add_method): (s':vstore{store_contains s' a}) =
+  fun a' -> if a' = a then Some (SP v am) else s a'
 
 (* per-thread verifier state *)
 noeq type vthread_state = 
   | VerifierThread: store:vstore -> clk:timestamp -> lk:merkle_addr -> vthread_state
-
-(* get the store of a thread *)
-let thread_store (ts: vthread_state): vstore = VerifierThread?.store ts
-
-(* update the store of a thread *)
-let thread_store_update (ts: vthread_state)
-                        (a:merkle_addr{store_contains (thread_store ts) a})
-                        (v:merkle_payload_of_addr a): 
-  Tot (ts': vthread_state{store_contains (thread_store ts') a /\
-                          stored_payload (thread_store ts') a = v}) = 
-  match ts with
-  | VerifierThread store clk lk -> 
-    VerifierThread (store_update store a v) clk lk
 
 type vglobal_state = 
   | VerifierGlobal: hadd0:ms_hash_value ->
@@ -79,64 +89,131 @@ type vglobal_state =
 (* verifier state aggregated across all verifier threads *)
 noeq type vstate (p:nat) = 
   | Failed: vstate p
-  | Valid: ts:seq vthread_state{length ts = p} ->  (* thread-specific state *)
+  | Valid: tss:seq vthread_state{length tss = p} ->  (* thread-specific state *)
            gs:vglobal_state ->                     (* global state *)
            vstate p
 
-let verifier_read (#p:nat) (a:addr) (v:payload) 
-                  (tid:nat {tid < p}) 
-                  (vs: vstate p{Valid? vs}): vstate p = 
-  (* thread state *)
-  let ts = index (Valid?.ts vs) tid in
-  (* thread store *)
-  let store = VerifierThread?.store ts in
+(* verifier read operation; return false on verification failure *)
+let verifier_read (a:addr) (v:payload) 
+                  (store: vstore): bool =
   (* merkle addr *)
   let ma = addr_to_merkle_leaf a in
   (* check store contains addr *)
-  let optPayload = store ma in
+  if not (store_contains store ma) then false
+  (* check stored payload is v *)
+  else stored_payload store ma = MkLeaf v
 
-  match optPayload with
-  | None -> Failed
-  | Some v' -> if v = MkLeaf?.value v' then vs 
-               else Failed      
-
-let verifier_write (#p:nat) (a:addr) (v:payload)
-                   (tid:nat {tid < p}) 
-                   (vs: vstate p{Valid? vs}): vstate p = 
-  (* thread state *)
-  let ts = index (Valid?.ts vs) tid in
-  (* thread store *)
-  let store = VerifierThread?.store ts in
+(* verification write operation: return updated store on success; Null on failure *)
+let verifier_write (a:addr) (v:payload)
+                   (store: vstore): option vstore = 
   (* merkle addr *)
-  let ma = addr_to_merkle_leaf a in
+  let ma = addr_to_merkle_leaf a in  
   (* check store contains addr *)
-  let optPayload = store ma in
+  if not (store_contains store ma) then None
+  (* update the store *)
+  else Some (store_update store ma (MkLeaf v))
 
-  match optPayload with
-  | None -> Failed
-  | Some _ -> admit() 
+let is_empty_or_null (a:merkle_addr) (v:merkle_payload_of_addr a): Tot bool =
+  if is_merkle_leaf a then Null? (MkLeaf?.value v)
+  else Empty? (MkInternal?.left v) &&
+       Empty? (MkInternal?. right v)
+
+let update_desc_hash (v:merkle_payload_internal)
+                     (d:bin_tree_dir)
+                     (a:merkle_addr)
+                     (h:hash_value) =
+  match v with
+  | MkInternal dhl dhr -> match d with 
+                         | Left -> MkInternal (Desc a h false) dhr
+                         | Right -> MkInternal dhl (Desc a h false)
+
+let verifier_addm (s: vstore) 
+                  (a: merkle_addr)
+                  (v: merkle_payload)
+                  (a': merkle_addr): option vstore = 
+  (* check a is a proper desc of a' *)                  
+  if not (is_proper_desc a a') then None
+  (* check store contains a' *)
+  else if not (store_contains s a') then None
+  (* check store does not contain a *)
+  else if store_contains s a then None 
+  (* Check the payload type corresponds to leaf/internal ness of address a *)
+  else if not (is_payload_of_addr a v) then None
+  
+  else (
+    let v' = stored_payload s a' in
+    let d = desc_dir a a' in
+
+    lemma_proper_desc_depth_monotonic a a';
+    assert(not (is_merkle_leaf a'));
+    
+    let dh' = desc_hash_dir d v' in
+    let h = hashfn v in
+
+    match dh' with
+    | Empty -> if (is_empty_or_null a v) then 
+                 let v'_upd = update_desc_hash v' d a h in
+                 let s_upd = store_update s a' v'_upd in
+                 Some (store_add s_upd a v Merkle)
+               else None
+    | Desc a2 h2 b2 -> if a2 = a && h2 = h then Some (store_add s a v Merkle) 
+                       else if not (is_empty_or_null a v) then None                        
+                       else if not (is_proper_desc a2 a) then None
+                       else (
+                         lemma_proper_desc_depth_monotonic a2 a;
+                         assert(not (is_merkle_leaf a));
+
+                         let d2 = desc_dir a2 a in
+                         let v_upd = update_desc_hash v d2 a2 h2 in
+                         let v'_upd = update_desc_hash v' d a h in
+                         let s_upd = store_update s a' v'_upd in
+                         Some (store_add s_upd a v Merkle)
+                       )
+  )    
+  
+
+(* update the store of a specific thread *)
+let thread_update_store (#p:nat) (tid:nat {tid < p}) 
+                        (vs:vstate p{Valid? vs})
+                        (store:vstore): vstate p = 
+  let tss = Valid?.tss vs in
+  let gs = Valid?.gs vs in
+  let ts = index tss tid in
+  match ts with
+  | VerifierThread _ clk lk -> 
+    let ts_upd = VerifierThread store clk lk in
+    let tss_upd = upd tss tid ts_upd in
+    Valid tss_upd gs
 
 let verifier_step_thread (#p:nat) 
                          (e:vlog_entry_thread) 
                          (tid:nat {tid < p}) 
                          (vs:vstate p{Valid? vs}): vstate p = 
-  // thread state                         
-  let ts = index (Valid?.ts vs) tid in
-  // global state
   let gs = Valid?.gs vs in
-  // thread store
+  let tss = Valid?.tss vs in
+  let ts = index tss tid in
   let store = VerifierThread?.store ts in
   match e with
   | MemoryOp o -> 
     (
     match o with
-    | Read a v -> verifier_read a v tid vs      
-    | Write a v -> admit()
+    | Read a v -> if verifier_read a v store       
+                  then vs
+                  else Failed
+    | Write a v -> let optStore = verifier_write a v store in
+                   match optStore with
+                   | None -> Failed
+                   | Some store' -> thread_update_store tid vs store'    
     )
-  | AddM _ _ _ -> 
-    admit()
+  | AddM a v a' -> let optStore = verifier_addm store a v a' in
+                   (
+                     match optStore with
+                     | None -> Failed
+                     | Some store' -> thread_update_store tid vs store'
+                   )
   | EvictM _ _ ->
     admit()
+  | _ -> admit()
 
 let verifier_step (#p:nat) (e:vlog_entry) (vs:vstate p): vstate p = 
   match vs with
